Weidenbach_Book/IsaSAT_Show.thy
@@ -75,11 +75,11 @@ lemma print_current_information_isasat_current:
 
 definition isasat_current_status :: \<open>twl_st_wl_heur \<Rightarrow> twl_st_wl_heur nres\<close> where
 \<open>isasat_current_status =
-   (\<lambda>(M', N', D', j, W', vm, \<phi>, clvls, cach, lbd, outl, stats,
+   (\<lambda>(M', N', D', j, W', vm, clvls, cach, lbd, outl, stats,
        heur, avdom,
        vdom, lcount, opts, old_arena).
      let stats = (print_current_information stats lcount)
-     in RETURN (M', N', D', j, W', vm, \<phi>, clvls, cach, lbd, outl, stats,
+     in RETURN (M', N', D', j, W', vm, clvls, cach, lbd, outl, stats,
        heur, avdom,
        vdom, lcount, opts, old_arena))\<close>
 
